src/Eqvivalence/BsFs/Helpers.v
@@ -754,7 +754,7 @@ End EnvironmentLemmas_GetValue.
 
 
 
-
+(* 
 
 Section EnvironmentLemmas_Remove.
 
@@ -793,7 +793,7 @@ Section EnvironmentLemmas_Remove.
 
 
 End EnvironmentLemmas_Remove.
-
+ *)
 
 
 
@@ -811,7 +811,7 @@ End EnvironmentLemmas_Remove.
 ////////////////////////////////////////////////////////////////////////////////
 *)
 
-
+(* 
 Section EraserLemmas.
 
 
@@ -847,7 +847,7 @@ Section EraserLemmas.
 
 End EraserLemmas.
 
-
+ *)
 
 
 
@@ -870,7 +870,7 @@ Section EraserSubstAppend_EraserLemmas.
 
 
 
-  Lemma add_keys_app :
+ (*  Lemma add_keys_app :
     forall keys1 keys2 σ,
       add_keys keys1 (add_keys keys2 σ)
     = add_keys (keys1 ++ keys2) σ.
@@ -879,7 +879,7 @@ Section EraserSubstAppend_EraserLemmas.
     ufl - add_keys.
     unfold add_names.
     bwr - foldr_app.
-  Qed.
+  Qed. *)
 
 
 
@@ -892,7 +892,7 @@ Section EraserSubstAppend_EraserLemmas.
     ufl - get_env.
     rwr - map_app.
     rwr - ext_to_env_fst.
-    rwl - add_keys_app.
+    rwr - add_keys_app.
     ufl - add_ext add_fids.
     bwr - map_map.
   Qed.
@@ -908,7 +908,7 @@ Section EraserSubstAppend_EraserLemmas.
     itr - vars vs Γ σ Hlength.
     ufl - append_vars_to_env.
     rwr - map_app.
-    rwl - add_keys_app.
+    rwr - add_keys_app.
     epose proof length_map (inl : Var -> (Var + FunctionIdentifier)) vars
       as Hlength_map_inl.
     cwl - Hlength_map_inl in Hlength.
@@ -917,6 +917,21 @@ Section EraserSubstAppend_EraserLemmas.
     cwr - Hzip_fst.
     ufl - add_vars.
     trv.
+  Qed.
+
+
+
+  Lemma from_env_append_vars_to_env_app :
+    forall vars vs Γ,
+        length vars = length vs
+    ->  from_env (append_vars_to_env vars vs Γ)
+      = add_vars vars (from_env Γ).
+  Proof.
+    itr - vars vs Γ Hlength.
+    ufl - from_env
+          add_env.
+    app - add_keys_append_vars_to_env_app.
+    exa - Hlength.
   Qed.
 
 
@@ -1016,48 +1031,42 @@ Section EraserSubstAppend_Theorems.
 
 
 
-  Theorem erase_exp_append_vars :
-    forall e fns env vars vs,
+
+  Theorem erase_subst_append_vars :
+    forall Γ vars e vs,
         base.length vars = base.length vs
     ->  (erase_exp
-          (add_keys
-            (map fst (append_vars_to_env vars vs env))
-            fns)
+          (from_env (append_vars_to_env vars vs Γ))
           e)
         .[list_subst
           (map
-            (fun v => erase_val (measure_val v) fns v)
-            (map snd (append_vars_to_env vars vs env)))
+            (fun v => erase_val' v)
+            (map snd (append_vars_to_env vars vs Γ)))
           idsubst]
       = (erase_exp
-          (add_vars
-            vars
-            (add_keys (map fst env) fns))
+          (add_vars vars (from_env Γ))
           e)
-        .[upn
-          (base.length vars)
+        .[upn (base.length vars)
           (list_subst
             (map
-               (fun v =>
-                 erase_val 
-                 (measure_val v) fns v)
-               (map snd env)) idsubst)]
+               (fun v => erase_val' v)
+               (map snd Γ)) idsubst)]
         .[list_subst
           (map
-            (fun v => erase_val (measure_val v) fns v) vs)
+            (fun v => erase_val' v) vs)
             idsubst].
   Proof.
-    itr - e fns env vars vs Hlength.
+    itr -  Γ vars e vs Hlen.
     (* add_keys *)
-    rwr - add_keys_append_vars_to_env_app.
+    rwr - from_env_append_vars_to_env_app.
     (* upn to ++ *)
     rwr - subst_comp_exp.
     ass >
       (length vs
-        = length (map (λ v : Value, erase_val (measure_val v) fns v) vs))
+        = length (map (fun v => erase_val' v) vs))
       as Hlength_vars:
       rwr - length_map.
-    rwl - Hlength in Hlength_vars.
+    rwl - Hlen in Hlength_vars.
     cwr - Hlength_vars.
     rwr - substcomp_list.
     rwr - substcomp_id_l.
@@ -1068,9 +1077,9 @@ Section EraserSubstAppend_Theorems.
     epose proof length_map (inl : Var -> (Var + FunctionIdentifier)) vars
       as Hlength_map_inl.
     2: asm.
-    cwl - Hlength_map_inl in Hlength.
-    epose proof zip_snd _ _ _ _ Hlength as Hzip_snd;
-      clr - Hlength.
+    cwl - Hlength_map_inl in Hlen.
+    epose proof zip_snd _ _ _ _ Hlen as Hzip_snd;
+      clr - Hlen.
     rwr - Hzip_snd.
     bwr - map_app.
   Qed.
@@ -1143,29 +1152,49 @@ Section Axioms_Definitions.
 
 
 
-Axiom all_val_is_wfm :
-  forall v,
-    wfm_fs_val v.
+  Axiom all_val_is_wfm :
+    forall v,
+      wfm_fs_val v.
 
 
 
-Axiom no_modfunc :
-  forall fid modules own_module,
-    get_own_modfunc own_module fid.1 fid.2 (modules ++ stdlib) = None.
+  Axiom no_modfunc :
+    forall modules own_module fid,
+      get_own_modfunc own_module fid.1 fid.2 (modules ++ stdlib) = None.
 
 
 
-Axiom result_is_result :
-  forall Γ modules own_module id id' e res eff eff' σ,
-      (eval_expr Γ modules own_module id e eff id' res eff')
-  ->  is_result (erase_result σ res).
+  Axiom result_is_result :
+    forall Γ modules own_module e r id id' eff eff',
+        (eval_expr Γ modules own_module id e eff id' r eff')
+    ->  is_result (erase_result r).
 
 
-(* refactor *)
-Axiom eval_fun_rem_vars :
-  forall vars e Γ modules own_module id res eff,
-      (eval_expr Γ modules own_module id (EFun vars e) eff (S id) res eff)
-  ->  rem_vars vars Γ = Γ.
+
+  Axiom eval_catch_vars_length :
+    forall Γ modules own_module vars1 vars2 e1 e2 e3 r id id' eff eff',
+        (eval_expr Γ modules own_module id (ETry e1 vars1 e2 vars2 e3) eff id' r eff')
+    ->  length vars2 = 3.
+
+
+
+  Axiom erase_subst_rem_vars :
+    forall Γ vars e,
+       (erase_exp
+        (add_vars vars (add_env (rem_vars vars Γ) σ0))
+        e)
+      .[upn (base.length vars)
+        (list_subst
+          (map erase_val' (map snd (rem_vars vars Γ)))
+          idsubst)]
+    = (erase_exp
+        (add_vars vars (add_env Γ σ0))
+        e)
+      .[upn (base.length vars)
+        (list_subst
+          (map erase_val' (map snd Γ))
+          idsubst)].
+
 
 
 End Axioms_Definitions.
@@ -1183,33 +1212,29 @@ Section Axioms_Lemmas.
 
 
   Lemma get_value_is_result :
-    forall key v Γ σ
-      (modules : list ErlModule) (own_module : string) (id : nat)
-      (eff : SideEffectList),
+    forall  Γ (modules : list ErlModule) (own_module : string)
+            key v (id : nat) (eff : SideEffectList),
         get_value Γ key = Some [v]
-    ->  VALCLOSED (erase_val (measure_val v) σ v).
+    ->  VALCLOSED (erase_val' v).
   Proof.
-    itr - key v Γ σ modules own_module id eff Hget.
-    ass >
-      (is_result
-        (RValSeq (map (fun v' => erase_val (measure_val v') σ v') [v])))
-      as Hscope.
+    itr - Γ modules own_module key v id eff Hget.
+    ass > (is_result (RValSeq (map (fun v' => erase_val' v') [v]))) as Hscope.
     {
-      rem - res as Hres:
-        (inl [v] : ValueSequence + Exception).
+      rem - r as Hr:
+            (inl [v] : ValueSequence + Exception).
       des - key as [var | fid].
       * rem - e as He:
-          (EVar var).
+              (EVar var).
         pse - result_is_result as Hresult:
-          Γ modules own_module id id e res eff eff σ.
+              Γ modules own_module e r id id eff eff.
         sbt.
         app - Hresult.
         clr - Hresult.
         bpp - eval_var.
       * rem - e as He:
-          (EFunId fid).
+              (EFunId fid).
         pse - result_is_result as Hresult:
-          Γ modules own_module id id e res eff eff σ.
+              Γ modules own_module e r id id eff eff.
         sbt.
         app - Hresult.
         clr - Hresult.
@@ -1223,68 +1248,89 @@ Section Axioms_Lemmas.
 
 
 
-  Lemma var_is_result :
-    forall var vs Γ σ
-      (modules : list ErlModule) (own_module : string) (id : nat)
-      (eff : SideEffectList),
+  Lemma evar_is_result :
+    forall  Γ (modules : list ErlModule) (own_module : string)
+            var vs (id : nat) (eff : SideEffectList),
         get_value Γ (inl var) = Some vs
     ->  (exists v,
             [v] = vs
-        /\  VALCLOSED (erase_val (measure_val v) σ v)).
+        /\  VALCLOSED (erase_val' v)).
   Proof.
-    itr - var vs Γ σ modules own_module id eff Hget.
-    rem - key as Hkey: (inl var : Var + FunctionIdentifier).
-    pse - get_value_singleton as Hsingle: Γ key vs Hget.
+    itr - Γ modules own_module var vs id eff Hget.
+    rem - key as Hkey:
+          (inl var : Var + FunctionIdentifier).
+    pse - get_value_singleton as Hsingle:
+          Γ key vs Hget.
     des - Hsingle as [v Hsingle].
     cwr - Hsingle in *; clr - vs.
     exi - v.
     spl.
     rfl.
     pse - get_value_is_result as Hscope:
-      key v Γ σ modules own_module id eff Hget.
+          Γ modules own_module key v id eff Hget.
     exa - Hscope.
   Qed.
 
 
 
-  Lemma funid_is_result :
-    forall fid vs Γ σ
-      (modules : list ErlModule) (own_module : string) (id : nat)
-      (eff : SideEffectList),
+  Lemma efunid_is_result :
+    forall  Γ (modules : list ErlModule) (own_module : string)
+            fid vs (id : nat) (eff : SideEffectList),
         get_value Γ (inr fid) = Some vs
     ->  (exists v,
             [v] = vs
-        /\  VALCLOSED (erase_val (measure_val v) σ v)).
+        /\  VALCLOSED (erase_val' v)).
   Proof.
-    itr - fid vs Γ σ modules own_module id eff Hget.
-    rem - key as Hkey: (inr fid : Var + FunctionIdentifier).
-    pse - get_value_singleton as Hsingle: Γ key vs Hget.
+    itr - Γ modules own_module fid vs id eff Hget.
+    rem - key as Hkey:
+          (inr fid : Var + FunctionIdentifier).
+    pse - get_value_singleton as Hsingle:
+          Γ key vs Hget.
     des - Hsingle as [v Hsingle].
     cwr - Hsingle in *; clr - vs.
     exi - v.
     spl.
     rfl.
     pse - get_value_is_result as Hscope:
-      key v Γ σ modules own_module id eff Hget.
+          Γ modules own_module key v id eff Hget.
     exa - Hscope.
   Qed.
 
 
 
-  Lemma fun_is_result :
-    forall vars e id Γ σ
-      (modules : list ErlModule) (own_module : string) (eff : SideEffectList),
-        is_result (erase_result σ (inl [VClos Γ [] id vars e]))
-    /\  rem_vars vars Γ = Γ.
+  Lemma efun_is_result :
+    forall  Γ (modules : list ErlModule) (own_module : string)
+            vars e id (eff : SideEffectList),
+      is_result (erase_result (inl [VClos Γ [] id vars e])).
   Proof.
-    itr - vars e id Γ σ modules own_module eff.
-    pse - eval_fun as Heval: Γ modules own_module vars e eff id.
-    spl.
-    * bse - result_is_result: Γ modules own_module id (S id)
-        (EFun vars e) (inl [VClos Γ [] id vars e] : ValueSequence + Exception)
-        eff eff σ Heval.
-    * bse - eval_fun_rem_vars: vars e Γ modules own_module id
-        (inl [VClos Γ [] id vars e] : ValueSequence + Exception) eff Heval.
+    itr - Γ modules own_module vars e id eff.
+    pse - eval_fun as Heval:
+          Γ modules own_module vars e eff id.
+    bse - result_is_result:
+          Γ modules own_module (EFun vars e)
+          (inl [VClos Γ [] id vars e] : ValueSequence + Exception)
+          id (S id) eff eff Heval.
+  Qed.
+
+
+
+  Lemma catch_vars_length :
+    forall Γ modules own_module (vars1 : list Var) vars2 e1 (e2 : Expression)
+           e3 x1 r3 id id' id'' eff eff' eff'',
+        eval_expr Γ modules own_module id e1 eff id' (inr x1) eff'
+    ->  eval_expr (append_vars_to_env vars2 (exc_to_vals x1) Γ)
+                  modules own_module id' e3 eff' id'' r3 eff''
+    ->  length vars2 = 3.
+  Proof.
+    itr - Γ modules own_module vars1 vars2 e1 e2 e3 x1 r3 id id' id''
+          eff eff' eff'' IHe1 IHe3.
+    rwl - exc_to_vals_eq in IHe3.
+    pse - eval_catch as Heval:
+          Γ modules own_module vars1 vars2 e1 e2 e3 r3
+          eff eff' eff'' id id' id'' x1 IHe1 IHe3.
+    bse - eval_catch_vars_length:
+          Γ modules own_module vars1 vars2 e1 e2 e3 r3
+          id id'' eff eff'' Heval.
   Qed.
 
 
